@prefix as: <https://www.w3.org/ns/activitystreams#> .
@prefix dc: <http://purl.org/dc/elements/1.1/> .
@prefix dcterms: <http://purl.org/dc/terms/> .
@prefix owl: <http://www.w3.org/2002/07/owl#> .
@prefix rdf: <http://www.w3.org/1999/02/22-rdf-syntax-ns#> .
@prefix rdfs: <http://www.w3.org/2000/01/rdf-schema#> .
@prefix schema: <https://schema.org/> .
@prefix xsd: <http://www.w3.org/2001/XMLSchema#> .

<https://w3id.org/fep/8a8e/AttendeesCollection> a rdfs:Class ;
	rdfs:label "A Collection of the Event's attendees"@en ;
	rdfs:comment """
      Inherits all properties from https://www.w3.org/ns/activitystreams#Collection with the addition that the items may also include https://schema.org/Person or https://schema.org/Organization.
      The items of the AttendeesCollection are entities that are confirmed attendees by an Events organizer(s). It contains all ActivityPub actors that meet one or more of the following conditions, added as a side effect.
      
The actor has sent a Join activity with this object as the object property that has been answered with an Accept.
The actor has responded to an Invite activity from the Event's owner (where the Event is specified as the object property) with an Accept activity.

      The items MAY be filtered on privileges of an authenticated user or as appropriate when no authentication is given. This collection *SHOULD* have the totalItems set in any case.
    """@en ;
	rdfs:isDefinedBy <https://w3id.org/fep/8a8e> ;
	rdfs:seeAlso <https://w3id.org/fep/8a8e/attendees> ;
	rdfs:subClassOf as:OrderedCollection .

<https://w3id.org/fep/8a8e/EventCancelled> a rdfs:Class ;
	rdfs:label "The event has been cancelled."@en ;
	rdfs:comment "The event has been cancelled."@en ;
	rdfs:isDefinedBy <https://w3id.org/fep/8a8e> ;
	rdfs:seeAlso <https://w3id.org/fep/8a8e/EventPostponed>,
		<https://w3id.org/fep/8a8e/EventRescheduled>,
		<https://w3id.org/fep/8a8e/eventStatus> ;
	rdfs:subClassOf <https://w3id.org/fep/8a8e/EventStatusType> .

<https://w3id.org/fep/8a8e/EventMovedOnline> a rdfs:Class ;
	rdfs:label "The event moved online."@en ;
	rdfs:comment "Indicates that the event was changed to allow online participation."@en ;
	rdfs:isDefinedBy <https://w3id.org/fep/8a8e> ;
	rdfs:seeAlso <https://w3id.org/fep/8a8e/eventStatus> ;
	rdfs:subClassOf <https://w3id.org/fep/8a8e/EventStatusType> .

<https://w3id.org/fep/8a8e/EventPostponed> a rdfs:Class ;
	rdfs:label "The event has been postponed."@en ;
	rdfs:comment "The event has been postponed and no new date has been set. The event's previousStartTime should be set."@en ;
	rdfs:isDefinedBy <https://w3id.org/fep/8a8e> ;
	rdfs:seeAlso <https://w3id.org/fep/8a8e/eventStatus> ;
	rdfs:subClassOf <https://w3id.org/fep/8a8e/EventStatusType> .

<https://w3id.org/fep/8a8e/EventRescheduled> a rdfs:Class ;
	rdfs:label "The event has been rescheduled."@en ;
	rdfs:comment "The event's previousStartTime should be set to the old date and the startTime should be set to the event's new start date."@en ;
	rdfs:isDefinedBy <https://w3id.org/fep/8a8e> ;
	rdfs:seeAlso <https://w3id.org/fep/8a8e/eventStatus> ;
	rdfs:subClassOf <https://w3id.org/fep/8a8e/EventStatusType> .

<https://w3id.org/fep/8a8e/EventScheduled> a rdfs:Class ;
	rdfs:label "The event is scheduled."@en ;
	rdfs:comment "The event is normally scheduled and planned."@en ;
	rdfs:isDefinedBy <https://w3id.org/fep/8a8e> ;
	rdfs:seeAlso <https://w3id.org/fep/8a8e/eventStatus> ;
	rdfs:subClassOf <https://w3id.org/fep/8a8e/EventStatusType> .

<https://w3id.org/fep/8a8e/EventStatusType> a rdfs:Class ;
	rdfs:label "8a8e"@en ;
	rdfs:comment "EventStatusType is an enumeration type whose instances represent several states that an Event may be in."@en ;
	rdfs:isDefinedBy <https://w3id.org/fep/8a8e> ;
	rdfs:seeAlso <https://w3id.org/fep/8a8e/eventStatus> ;
	rdfs:subClassOf schema:EventStatusType .

<https://w3id.org/fep/8a8e/EventTentative> a rdfs:Class ;
	rdfs:label "The event is tentative"@en ;
	rdfs:comment "The event is currently being planned but not confirmed."@en ;
	rdfs:isDefinedBy <https://w3id.org/fep/8a8e> ;
	rdfs:seeAlso <https://w3id.org/fep/8a8e/eventStatus> ;
	rdfs:subClassOf <https://w3id.org/fep/8a8e/EventStatusType> .

<https://w3id.org/fep/8a8e/OrganizersCollection> a rdfs:Class ;
	rdfs:label "An Event's Organizer Collection"@en ;
	rdfs:comment "Inherits all properties from https://www.w3.org/ns/activitystreams#Collection with the addition that the items may also include https://schema.org/Person or https://schema.org/Organization."@en ;
	rdfs:isDefinedBy <https://w3id.org/fep/8a8e> ;
	rdfs:seeAlso <https://w3id.org/fep/8a8e/organizers> ;
	rdfs:subClassOf as:Collection .

<https://w3id.org/fep/8a8e/category> a owl:DatatypeProperty ;
	rdfs:label "The category of an Event"@en ;
	rdfs:comment """Recommended event categories include: ARTS, AUTO_BOAT_AIR, BOOK_CLUBS, BUSINESS, CAUSES, CLIMATE_ENVIRONMENT, COMMUNITY, COMEDY, CRAFTS, CREATIVE_JAM, DIY_MAKER_SPACES, FAMILY_EDUCATION, FASHION_BEAUTY, FESTIVALS, FILM_MEDIA, FOOD_DRINK, GAMES, INCLUSIVE_SPACES, LANGUAGE_CULTURE, LEARNING, LGBTQ, MEETING, MEDITATION_WELLBEING, MOVEMENTS_POLITICS, MUSIC, NETWORKING, OUTDOORS_ADVENTURE, PARTY, PERFORMING_VISUAL_ARTS, PETS, PHOTOGRAPHY, SCIENCE_TECH, SPIRITUALITY_RELIGION_BELIEFS, SPORTS, THEATRE, WORKSHOPS_SKILL_SHARING
"""@en ;
	rdfs:domain as:Event ;
	rdfs:isDefinedBy <https://w3id.org/fep/8a8e> ;
	rdfs:range xsd:string .

<https://w3id.org/fep/8a8e/externalParticipationUrl> a owl:DatatypeProperty ;
	rdfs:label "External participation URL"@en ;
	rdfs:comment """
      A URL that points to an external platform where people can join the event or where they can buy tickets for the event. Required if joinMode is set to external.
    """@en ;
	rdfs:domain as:Event ;
	rdfs:isDefinedBy <https://w3id.org/fep/8a8e> ;
	rdfs:range xsd:anyURI .

<https://w3id.org/fep/8a8e/isBannerImage> a owl:DatatypeProperty ;
	rdfs:label "Image is a banner image"@en ;
	rdfs:comment """
      Whether an image is an (events) banner image.
    """@en ;
	rdfs:domain as:Image ;
	rdfs:isDefinedBy <https://w3id.org/fep/8a8e> ;
	rdfs:range xsd:boolean .

<https://w3id.org/fep/8a8e/joinMode> a owl:ObjectProperty ;
	rdfs:label "Join mode"@en ;
	rdfs:comment """
      Indicator of how new members may be able to join an event.
      Accepted values: free, restricted, external, none, invite.
      If external, you must also set externalParticipationUrl.
    """@en ;
	rdfs:domain as:Event ;
	rdfs:isDefinedBy <https://w3id.org/fep/8a8e/> ;
	rdfs:range xsd:string .

<https://w3id.org/fep/8a8e/previousStartTime> a owl:DatatypeProperty ;
	rdfs:label "The event previous start time."@en ;
	rdfs:comment "The events previous start time is the old start time before an event got postponed or rescheduled."@en ;
	rdfs:domain as:Event ;
	rdfs:isDefinedBy <https://w3id.org/fep/8a8e> ;
	rdfs:range xsd:dateTime ;
	rdfs:seeAlso <https://w3id.org/fep/8a8e/EventPostponed>,
		<https://w3id.org/fep/8a8e/EventRescheduled> .

<https://w3id.org/fep/8a8e/requiredJoinVisibility> a owl:ObjectProperty ;
	rdfs:label "Required Join Visibility"@en ;
	rdfs:comment """
      Specifies the minimum audience that must be addressed in a valid Join activity related to the event. This can include individual actors, groups, the as:Public collection, or any other URI. The Join activity must be addressed accordingly (e.g., using to, cc, bto, or audience).
    """@en ;
	rdfs:domain as:Event ;
	rdfs:isDefinedBy <https://w3id.org/fep/8a8e> ;
	rdfs:range xsd:anyURI .

<https://w3id.org/fep/8a8e/timezone> a owl:ObjectProperty ;
	rdfs:label "The timezone of an Event"@en ;
	rdfs:comment "Indicates the timezone for which the time(s) indicated in the event are given. The value provided should be among those listed in the IANA Time Zone Database."@en ;
	rdfs:isDefinedBy <https://w3id.org/fep/8a8e> ;
	rdfs:range rdfs:Literal .

<https://w3id.org/fep/8a8e/upcomingEvents> a owl:ObjectProperty ;
	rdfs:label "Ordered collection of upcoming Events"@en ;
	rdfs:comment "An ActivityStreams OrderedCollection of Event objects that have a startTime property in the future, sorted by startTime with the earliest first."@en ;
	rdfs:isDefinedBy <https://w3id.org/fep/8a8e> ;
	rdfs:range as:OrderedCollection .

<https://w3id.org/fep/8a8e/attendees> a owl:ObjectProperty ;
	rdfs:label "Attendees of an Event"@en ;
	rdfs:comment ""@en ;
	rdfs:isDefinedBy <https://w3id.org/fep/8a8e> ;
	rdfs:range rdfs:Resource ;
	owl:minCardinality "0"^^xsd:nonNegativeInteger .

<https://w3id.org/fep/8a8e/displayEndTime> a owl:DatatypeProperty ;
	rdfs:label "Whether to display the endTime"@en ;
	rdfs:comment "A property that defines whether the end time of an event should be displayed."@en ;
	rdfs:domain <https://w3id.org/fep/8a8e/displayEndTime> ;
	rdfs:isDefinedBy <https://w3id.org/fep/8a8e> ;
	rdfs:range xsd:boolean .

<https://w3id.org/fep/8a8e/organizers> a owl:ObjectProperty ;
	rdfs:label "Organizers Collection"@en ;
	rdfs:comment "An ActivityStreams Collection collection that lists the entities that are disclosed to as organizers of an event. If set to null this explicitly indicates a deliberate choice to withhold organizer information."@en ;
	rdfs:isDefinedBy <https://w3id.org/fep/8a8e> ;
	rdfs:range <https://w3id.org/fep/8a8e/OrganizersCollection> .

<https://w3id.org/fep/8a8e/eventStatus> a rdf:Property ;
	rdfs:label "The events status is"@en ;
	rdfs:comment "An eventStatus of an event represents its status; particularly useful when an event is cancelled or rescheduled."@en ;
	rdfs:domain as:Event ;
	rdfs:isDefinedBy <https://w3id.org/fep/8a8e> ;
	rdfs:range <https://w3id.org/fep/8a8e/EventStatusType> ;
	rdfs:seeAlso <https://w3id.org/fep/8a8e/EventCancelled>,
		<https://w3id.org/fep/8a8e/EventMovedOnline>,
		<https://w3id.org/fep/8a8e/EventPostponed>,
		<https://w3id.org/fep/8a8e/EventRescheduled>,
		<https://w3id.org/fep/8a8e/EventScheduled>,
		<https://w3id.org/fep/8a8e/EventTentative> ;
	owl:maxCardinality "1"^^xsd:nonNegativeInteger ;
	owl:minCardinality "0"^^xsd:nonNegativeInteger .

<https://w3id.org/fep/8a8e> a owl:Ontology ;
	dc:creator "Andr√© Menrath <andre.menrath@posteo.de>",
		"les <lesion@autistici.org>" ;
	dc:rights "CC0 1.0 Universal (CC0 1.0) Public Domain Dedication"@en ;
	dcterms:abstract "ActivityStreams defines the Object Type Event. In real-world applications, the event object immediately showed the need for extension. Applications featuring Event objects have often chosen to add additional attributes and clarifications (i.e., interpretations) in order to implement their particular use case. This proposal clarifies and extends the ActivityPub standard to address the needs that have arisen in real-world implementations." ;
	dcterms:dateSubmitted "2025-04-23"^^xsd:date ;
	dcterms:identifier "https://w3id.org/fep/8a8e"^^xsd:anyURI ;
	dcterms:license <https://creativecommons.org/publicdomain/zero/1.0/> ;
	dcterms:title "FEP-8a8e: A common approach to using the Event object type" .

