@prefix as: <https://www.w3.org/ns/activitystreams#> .
@prefix dc: <http://purl.org/dc/elements/1.1/> .
@prefix dcterms: <http://purl.org/dc/terms/> .
@prefix owl: <http://www.w3.org/2002/07/owl#> .
@prefix rdfs: <http://www.w3.org/2000/01/rdf-schema#> .
@prefix xsd: <http://www.w3.org/2001/XMLSchema#> .

<https://w3id.org/fep/888d#ExcludedExample> a rdfs:Class ;
	rdfs:label "Excluded Example"@en ;
	rdfs:comment "A class that is useful for ontology but not intended to be used for the context mapping"@en ;
	rdfs:isDefinedBy <https://w3id.org/fep/888d> ;
	rdfs:subClassOf as:Object .

<https://w3id.org/fep/888d/SomeType> a rdfs:Class ;
	rdfs:label "Some Type"@en ;
	rdfs:comment "Some type."@en ;
	rdfs:isDefinedBy <https://w3id.org/fep/888d> ;
	rdfs:seeAlso <https://w3id.org/fep/888d/exampleA>,
		<https://w3id.org/fep/888d/exampleB>,
		<https://w3id.org/fep/888d/exampleC> ;
	rdfs:subClassOf as:Object .

<https://w3id.org/fep/888d/exampleA> a owl:DatatypeProperty ;
	rdfs:label "has example relation A with the literal value"@en ;
	rdfs:comment "A property with some literal value (string, boolean, number)"@en ;
	rdfs:domain <https://w3id.org/fep/888d/SomeType> ;
	rdfs:isDefinedBy <https://w3id.org/fep/888d> ;
	rdfs:range rdfs:Literal ;
	owl:maxCardinality "1"^^xsd:nonNegativeInteger ;
	owl:minCardinality "1"^^xsd:nonNegativeInteger .

<https://w3id.org/fep/888d/exampleB> a owl:ObjectProperty ;
	rdfs:label "has example relation B with"@en ;
	rdfs:comment "A property that links to another node on the graph (for example, another object)"@en ;
	rdfs:domain <https://w3id.org/fep/888d/SomeType> ;
	rdfs:isDefinedBy <https://w3id.org/fep/888d> ;
	rdfs:range rdfs:Resource ;
	owl:minCardinality "0"^^xsd:nonNegativeInteger .

<https://w3id.org/fep/888d/exampleC> a owl:DatatypeProperty ;
	rdfs:label "has an exampleC value of"@en ;
	rdfs:comment "A property that is an ordered list of literal values that are specifically non-negative integers"@en ;
	rdfs:domain <https://w3id.org/fep/888d/SomeType> ;
	rdfs:isDefinedBy <https://w3id.org/fep/888d> ;
	rdfs:range xsd:nonNegativeInteger ;
	owl:maxCardinality "1"^^xsd:nonNegativeInteger ;
	owl:minCardinality "0"^^xsd:nonNegativeInteger .

<https://w3id.org/fep/888d> a owl:Ontology ;
	dc:creator "a <a@trwnh.com>" ;
	dc:rights "CC0 1.0 Universal (CC0 1.0) Public Domain Dedication"@en ;
	dcterms:abstract "It is considered best practice in the linked-data ecosystem to have IRIs be HTTPS URIs that resolve to a definition of the term being used, and it is desirable to define such terms in a JSON-LD context file that is referenced by its IRI rather than having the full @context object embedded in every single document. ActivityStreams 2.0 and ActivityPub do this with the normative context and namespace provided at https://www.w3.org/ns/activitystreams, but this namespace is not generally open to extensions or to experimental terms. This FEP therefore proposes using https://w3id.org/fep as a base IRI for the FEP process, allowing sub-namespaces for each FEP." ;
	dcterms:dateSubmitted "2023-04-10"^^xsd:date ;
	dcterms:identifier "https://w3id.org/fep/888d"^^xsd:anyURI ;
	dcterms:license <https://creativecommons.org/publicdomain/zero/1.0/> ;
	dcterms:title "FEP-888d: Using https://w3id.org/fep as a base for FEP-specific namespaces" .

